erasure/theories/SafeTemplateErasure.v
@@ -142,11 +142,11 @@ Program Fixpoint check_wf_env_only_univs (Σ : global_env)
 From MetaCoq.Erasure Require Import SafeErasureFunction.
 
 Program Definition erase_template_program (p : Ast.program)
-  : EnvCheck (EAst.global_context * EAst.term) :=
+  : (EAst.global_context * EAst.term) :=
   let Σ := (trans_global (Ast.empty_ext p.1)).1 in
-  Σ' <- (SafeErasureFunction.erase_global Σ _) ;;
-  t <- wrap_error (empty_ext Σ) ("During erasure of " ^ string_of_term (trans p.2)) (SafeErasureFunction.erase (empty_ext Σ) _ nil (trans p.2) _);;
-  ret (Monad:=envcheck_monad) (Σ', t).
+  let Σ' := SafeErasureFunction.erase_global Σ _ in
+  let t := SafeErasureFunction.erase (empty_ext Σ) _ nil (trans p.2) _ in
+  (Σ', t).
 
 Next Obligation.
   unfold trans_global.
@@ -183,17 +183,12 @@ Program Definition erase_and_print_template_program_check {cf : checker_flags} (
 
 (** This uses the retyping-based erasure *)
 Program Definition erase_and_print_template_program {cf : checker_flags} (p : Ast.program)
-  : string + string :=
+  : string :=
   let p := fix_program_universes p in
-  match erase_template_program p return string + string with
-  | CorrectDecl (Σ', t) =>
-    inl ("Environment is well-formed and " ^ Pretty.print_term (Ast.empty_ext p.1) [] true p.2 ^
-         " erases to: " ^ nl ^ print_term Σ' [] true false t)
-  | EnvError Σ' (AlreadyDeclared id) =>
-    inr ("Already declared: " ^ id)
-  | EnvError Σ' (IllFormedDecl id e) =>
-    inr ("Type error: " ^ PCUICSafeChecker.string_of_type_error Σ' e ^ ", while checking " ^ id)
-  end.
+  let (Σ', t) := erase_template_program p in
+  "Environment is well-formed and " ^ Pretty.print_term (Ast.empty_ext p.1) [] true p.2 ^
+  " erases to: " ^ nl ^ print_term Σ' [] true false t.
+  
 
 (* Program Definition check_template_program {cf : checker_flags} (p : Ast.program) (ty : Ast.term) *)
 (*   : EnvCheck (∥ trans_global (AstUtils.empty_ext (List.rev p.1)) ;;; [] |- trans p.2 : trans ty ∥) := *)
